VCVio.lean
@@ -56,7 +56,7 @@ import VCVio.CryptoFoundations.MerkleTree.Inductive.Extractability
 import VCVio.CryptoFoundations.MerkleTree.Inductive.QueryBound
 import VCVio.CryptoFoundations.MerkleTree.Inductive.Uniqueness
 import VCVio.CryptoFoundations.MerkleTree.Addressed.Basic
-import VCVio.CryptoFoundations.MerkleTree.Tweaked.Basic
+import VCVio.CryptoFoundations.MerkleTree.Addressed.Level
 import VCVio.CryptoFoundations.MerkleTree.Vector.Completeness
 import VCVio.CryptoFoundations.MerkleTree.Vector.Defs
 import VCVio.CryptoFoundations.PRF
